src/Assembly/Conversions.v
@@ -61,25 +61,12 @@ Module HLConversions.
         convertExpr (f x y))
     end.
 
-  Fixpoint convertExpr' {A B: Type} {EA: Evaluable A} {EB: Evaluable B} {t} (a: expr (T := A) (var := @interp_type A) t): expr (T := B) (var := @interp_type B) t :=
-    match a with
-    | Const x => Const (@toT B EB (@fromT A EA x))
-    | Var t x => @Var B _ t (convertVar x)
-    | Binop t1 t2 t3 o e1 e2 =>
-      @Binop B _ t1 t2 t3 o (convertExpr' e1) (convertExpr' e2)
-    | Let tx e tC f =>
-      Let (convertExpr' e) (fun x => convertExpr' (f (convertVar x)))
-    | Pair t1 e1 t2 e2 => Pair (convertExpr' e1) (convertExpr' e2)
-    | MatchPair t1 t2 e tC f => MatchPair (convertExpr' e) (fun x y =>
-        convertExpr' (f (convertVar x) (convertVar y)))
-    end.
-
   Definition convertZToWord {t} n v a :=
-    @convertExpr Z (word n) ZEvaluable (@WordEvaluable n) t v a.
+    @convertExpr Z (word n) (@ZEvaluable n) (@WordEvaluable n) t v a.
 
   Definition convertZToBounded {t} n v a :=
     @convertExpr Z (option (@BoundedWord n))
-                 ZEvaluable (@BoundedEvaluable n) t v a.
+                 (@ZEvaluable n) (@BoundedEvaluable n) t v a.
 
   Definition ZToWord {t} n (a: @Expr Z t): @Expr (word n) t :=
     fun v => convertZToWord n v (a v).
@@ -97,316 +84,130 @@ Module HLConversions.
           Binop OPadd (Var x) (Var y)))))%Z.
 
   Example interp_example_range :
-    option_map high (BInterp (ZToRange 32 example_Expr)) = Some 28%N.
+    option_map bw_high (BInterp (ZToRange 32 example_Expr)) = Some 28%N.
   Proof. cbv; reflexivity. Qed.
 End HLConversions.
 
 Module LLConversions.
   Import LL.
 
-  Definition convertVar {A B: Type} {EA: Evaluable A} {EB: Evaluable B} {t} (a: interp_type (T := A) t): interp_type (T := B) t.
-  Proof.
-    induction t as [| t3 IHt1 t4 IHt2].
+  Section VarConv.
+    Context {A B: Type} {EA: Evaluable A} {EB: Evaluable B}.
 
-    - refine (@toT B EB (@fromT A EA _)); assumption.
+    Definition convertVar {t} (a: interp_type (T := A) t): interp_type (T := B) t.
+    Proof.
+      induction t as [| t3 IHt1 t4 IHt2].
 
-    - destruct a as [a1 a2]; constructor;
-        [exact (IHt1 a1) | exact (IHt2 a2)].
-  Defined.
+      - refine (@toT B EB (@fromT A EA _)); assumption.
 
-  Fixpoint convertArg {A B: Type} {EA: Evaluable A} {EB: Evaluable B} t {struct t}: @arg A A t -> @arg B B t :=
-    match t as t' return @arg A A t' -> @arg B B t' with
-    | TT => fun x =>
-      match x with
-      | Const c => Const (convertVar (t := TT) c)
-      | Var v => Var (convertVar (t := TT) v)
-      end
-    | Prod t0 t1 => fun x =>
-      match (match_arg_Prod x) with
-      | (a, b) => Pair ((convertArg t0) a) ((convertArg t1) b)
-      end
-    end.
+      - destruct a as [a1 a2]; constructor;
+          [exact (IHt1 a1) | exact (IHt2 a2)].
+    Defined.
+  End VarConv.
 
-  Arguments convertArg [_ _ _ _ _ _].
+  Section ArgConv.
+    Context {A B: Type} {EA: Evaluable A} {EB: Evaluable B}.
 
-  Fixpoint convertExpr {A B: Type} {EA: Evaluable A} {EB: Evaluable B} {t} (a: expr (T := A) t): expr (T := B) t :=
-    match a with
-    | LetBinop _ _ out op a b _ eC =>
-      LetBinop (T := B) op (convertArg a) (convertArg b) (fun x: (arg out) => convertExpr (eC (convertArg x)))
-    | Return _ a => Return (convertArg a)
-    end.
+    Fixpoint convertArg {V} t {struct t}: @arg A V t -> @arg B V t :=
+      match t as t' return @arg A V t' -> @arg B V t' with
+      | TT => fun x =>
+        match x with
+        | Const c => Const (convertVar (t := TT) c)
+        | Var v => Var v
+        end
+      | Prod t0 t1 => fun x =>
+        match (match_arg_Prod x) with
+        | (a, b) => Pair ((convertArg t0) a) ((convertArg t1) b)
+        end
+      end.
+  End ArgConv.
 
-  Definition convertZToWord {t} n a :=
-    @convertExpr Z (word n) ZEvaluable (@WordEvaluable n) t a.
+  Section ExprConv.
+    Context {A B: Type} {EA: Evaluable A} {EB: Evaluable B}.
 
-  Definition convertZToBounded {t} n a :=
-    @convertExpr Z (option (@BoundedWord n)) ZEvaluable (@BoundedEvaluable n) t a.
+    Fixpoint convertExpr {t V} (a: @expr A V t): @expr B V t :=
+        match a with
+        | LetBinop _ _ out op a b _ eC =>
+          LetBinop (T := B) op (convertArg _ a) (convertArg _ b) (fun x: (arg out) =>
+            convertExpr (eC (convertArg _ x)))
 
-  Definition zinterp {t} E := @interp Z ZEvaluable t E.
+        | Return _ a => Return (convertArg _ a)
+        end.
+  End ExprConv.
 
-  Definition wordInterp {n t} E := @interp (word n) (@WordEvaluable n) t E.
+  Section Defaults.
+    Context {t: type} {n: nat}.
 
-  Definition boundedInterp {n t} E: @interp_type (option (@BoundedWord n)) t :=
-    @interp (option (@BoundedWord n)) (@BoundedEvaluable n) t E.
+    Definition Word := word n.
+    Definition Bounded := option (@BoundedWord n).
+    Definition RWV := option (RangeWithValue).
+
+    Transparent Word Bounded RWV.
+
+    Instance RWVEvaluable' : Evaluable RWV := @RWVEvaluable n.
+    Instance ZEvaluable' : Evaluable Z := @ZEvaluable n.
+
+    Existing Instance ZEvaluable'.
+    Existing Instance WordEvaluable.
+    Existing Instance BoundedEvaluable.
+    Existing Instance RWVEvaluable'.
+
+    Definition ZToWord a := @convertExpr Z Word _ _ t a.
+    Definition ZToBounded a := @convertExpr Z Bounded _ _ t a.
+    Definition ZToRWV a := @convertExpr Z RWV _ _ t a.
+
+    Definition varZToWord a := @convertVar Z Word _ _ t a.
+    Definition varZToBounded a := @convertVar Z Bounded _ _ t a.
+    Definition varZToRWV a := @convertVar Z RWV _ _ t a.
+
+    Definition varWordToZ a := @convertVar Word Z _ _ t a.
+    Definition varBoundedToZ a := @convertVar Bounded Z _ _ t a.
+    Definition varRWVToZ a := @convertVar RWV Z _ _ t a.
+
+    Definition zinterp E := @interp Z _ t E.
+    Definition wordInterp E := @interp' Word _ _ t (fun x => NToWord n (Z.to_N x)) E.
+    Definition boundedInterp E := @interp Bounded _ t E.
+    Definition rwvInterp E := @interp RWV _ t E.
+
+    Section Operations.
+      Context {tx ty tz: type}.
+
+      Definition opZ (op: binop tx ty tz)
+                 (x: @interp_type Z tx) (y: @interp_type Z ty): @interp_type Z tz :=
+        @interp_binop Z _ _ _ _ op x y.
+
+      Definition opBounded (op: binop tx ty tz)
+                 (x: @interp_type Bounded tx) (y: @interp_type Bounded ty): @interp_type Bounded tz :=
+        @interp_binop Bounded _ _ _ _ op x y.
+
+      Definition opWord (op: binop tx ty tz)
+                 (x: @interp_type Word tx) (y: @interp_type Word ty): @interp_type Word tz :=
+        @interp_binop Word _ _ _ _ op x y.
+
+      Definition opRWV (op: binop tx ty tz)
+                 (x: @interp_type RWV tx) (y: @interp_type RWV ty): @interp_type RWV tz :=
+        @interp_binop RWV _ _ _ _ op x y.
+    End Operations.
+  End Defaults.
 
   Section Correctness.
-    (* Aliases to make the proofs easier to read. *)
-
-    Definition varZToBounded {n t} (v: @interp_type Z t): @interp_type (option (@BoundedWord n)) t :=
-      @convertVar Z (option (@BoundedWord n)) ZEvaluable BoundedEvaluable t v.
-
-    Definition varBoundedToZ {n t} (v: @interp_type _ t): @interp_type Z t :=
-      @convertVar (option (@BoundedWord n)) Z BoundedEvaluable ZEvaluable t v.
-
-    Definition varZToWord {n t} (v: @interp_type Z t): @interp_type (@word n) t :=
-      @convertVar Z (@word n) ZEvaluable (@WordEvaluable n) t v.
-
-    Definition varWordToZ {n t} (v: @interp_type (@word n) t): @interp_type Z t :=
-      @convertVar (word n) Z (@WordEvaluable n) ZEvaluable t v.
-
-    Definition zOp {tx ty tz: type} (op: binop tx ty tz)
-               (x: @interp_type Z tx) (y: @interp_type Z ty): @interp_type Z tz :=
-      @interp_binop Z ZEvaluable _ _ _ op x y.
-
-    Definition wOp {n} {tx ty tz: type} (op: binop tx ty tz)
-               (x: @interp_type _ tx) (y: @interp_type _ ty): @interp_type _ tz :=
-      @interp_binop (word n) (@WordEvaluable n) _ _ _ op x y.
-
-    Definition bOp {n} {tx ty tz: type} (op: binop tx ty tz)
-               (x: @interp_type _ tx) (y: @interp_type _ ty): @interp_type _ tz :=
-      @interp_binop (option (@BoundedWord n)) BoundedEvaluable _ _ _ op x y.
-
-    Definition boundedArg {n t} (x: @arg (option (@BoundedWord n)) (option (@BoundedWord n)) t) :=
-      @interp_arg _ _ x.
-
-    Definition wordArg {n t} (x: @arg (word n) (word n) t) := @interp_arg _ _ x.
-
-    (* BoundedWord-based Bounds-checking fixpoint *)
-
-    Definition getBounds {n t} T (E: Evaluable T) (e : @expr T T t): @interp_type (option (@BoundedWord n)) t :=
-      interp (E := BoundedEvaluable) (@convertExpr T (option (@BoundedWord n)) E BoundedEvaluable t e).
-
-    Fixpoint bcheck' {n t} (x: @interp_type (option (@BoundedWord n)) t) :=
-      match t as t' return (interp_type t') -> bool with
-      | TT => fun x' =>
-        match x' with
-        | Some _ => true
-        | None => false
-        end
-      | Prod t0 t1 => fun x' =>
-        match x' with
-        | (x0, x1) => andb (bcheck' x0) (bcheck' x1)
-        end
-      end x.
-
-    Definition bcheck {n t} T (E: Evaluable T) (e : @expr T T t): bool := bcheck' (n := n) (getBounds T E e).
-
-    (* Utility Lemmas *)
-
-    Lemma convertArg_interp: forall {A B t} {EA: Evaluable A} {EB: Evaluable B} (x: @arg A A t),
-        (interp_arg (@convertArg A B EA EB t x)) = @convertVar A B EA EB t (interp_arg x).
-    Proof.
-      induction x as [| |t0 t1 i0 i1]; [reflexivity|reflexivity|].
-      induction EA, EB; simpl; f_equal; assumption.
-    Qed.
-
-    Lemma convertArg_var: forall {A B EA EB t} (x: @interp_type A t),
-        @convertArg A B EA EB t (uninterp_arg x) = uninterp_arg (@convertVar A B EA EB t x).
-    Proof.
-      induction t as [|t0 IHt_0 t1 IHt_1]; simpl; intros; [reflexivity|].
-      induction x as [a b]; simpl; f_equal;
-        induction t0 as [|t0a IHt0_0 t0b IHt0_1],
-                  t1 as [|t1a IHt1_0]; simpl in *;
-        try rewrite IHt_0;
-        try rewrite IHt_1;
-        reflexivity.
-    Qed.
-
-    Ltac kill_just n :=
-      match goal with
-      | [|- context[just ?x] ] =>
-        let Hvalue := fresh in let Hvalue' := fresh in
-        let Hlow := fresh in let Hlow' := fresh in
-        let Hhigh := fresh in let Hhigh' := fresh in
-        let Hnone := fresh in let Hnone' := fresh in
-
-        let B := fresh in
-
-        pose proof (just_value_spec (n := n) x) as Hvalue;
-        pose proof (just_low_spec (n := n) x) as Hlow;
-        pose proof (just_high_spec (n := n) x) as Hhigh;
-        pose proof (just_None_spec (n := n) x) as Hnone;
-
-        destruct (just x);
-
-        try pose proof (Hlow _ eq_refl) as Hlow';
-        try pose proof (Hvalue _ eq_refl) as Hvalue';
-        try pose proof (Hhigh _ eq_refl) as Hhigh';
-        try pose proof (Hnone eq_refl) as Hnone';
-
-        clear Hlow Hhigh Hvalue Hnone
-      end.
-
-    Ltac kill_dec :=
-      repeat match goal with
-      | [|- context[Nge_dec ?a ?b] ] => destruct (Nge_dec a b)
-      | [H : context[Nge_dec ?a ?b] |- _ ] => destruct (Nge_dec a b)
-      end.
-
-    Lemma ZToBounded_binop_correct : forall {n tx ty tz} (op: binop tx ty tz) (x: arg tx) (y: arg ty) e,
-        bcheck (n := n) (t := tz) Z ZEvaluable (LetBinop op x y e) = true
-      -> zOp op (interp_arg x) (interp_arg y) =
-          varBoundedToZ (bOp (n := n) op (varZToBounded (interp_arg x)) (varZToBounded (interp_arg y))).
-    Proof.
-    Admitted.
-
-    Lemma ZToWord_binop_correct : forall {n tx ty tz} (op: binop tx ty tz) (x: arg tx) (y: arg ty) e,
-        bcheck (n := n) (t := tz) Z ZEvaluable (LetBinop op x y e) = true
-      -> zOp op (interp_arg x) (interp_arg y) =
-          varWordToZ (wOp (n := n) op (varZToWord (interp_arg x)) (varZToWord (interp_arg y))).
-    Proof.
-    Admitted.
-
-    Lemma just_zero: forall n, exists x, just (n := n) 0 = Some x.
-    Proof.
-    Admitted.
-
-    (* Main correctness guarantee *)
-
-    Lemma RangeInterp_bounded_spec: forall {n t} (E: expr t),
-        bcheck (n := n) Z ZEvaluable E = true
-      -> typeMap (fun x => NToWord n (Z.to_N x)) (zinterp E) = wordInterp (convertZToWord n E).
-    Proof.
-      intros n t E S.
-      unfold convertZToBounded, zinterp, convertZToWord, wordInterp.
-
-      induction E as [tx ty tz op x y z|]; simpl; try reflexivity.
-
-      - repeat rewrite convertArg_var in *.
-        repeat rewrite convertArg_interp in *.
-
-        rewrite H; clear H; repeat f_equal.
-
-        + pose proof (ZToWord_binop_correct (n := n) op x y) as C;
-            unfold zOp, wOp, varWordToZ, varZToWord in C;
-            simpl in C.
-
-          induction op; apply (C (fun _ => Return (Const 0%Z))); clear C;
-            unfold bcheck, getBounds; simpl;
-            destruct (@just_zero n) as [j p]; rewrite p; reflexivity.
-
-        + unfold bcheck, getBounds in *; simpl in *.
-          replace (interp_binop op _ _)
-             with (varBoundedToZ (n := n) (bOp (n := n) op
-                    (boundedArg (@convertArg _ _ ZEvaluable (@BoundedEvaluable n) _ x))
-                    (boundedArg (@convertArg _ _ ZEvaluable (@BoundedEvaluable n) _ y))));
-            [unfold varBoundedToZ, boundedArg; rewrite <- convertArg_var; assumption |].
-
-          pose proof (ZToBounded_binop_correct (n := n) op x y) as C;
-            unfold boundedArg, zOp, wOp, varZToBounded,
-                   varBoundedToZ, convertZToBounded in *;
-            simpl in C.
-
-          repeat rewrite convertArg_interp; symmetry.
-
-          induction op; apply (C (fun _ => Return (Const 0%Z))); clear C;
-            unfold bcheck, getBounds; simpl;
-            destruct (@just_zero n) as [j p]; rewrite p; reflexivity.
-
-      - simpl in S.
-        induction a as [| |t0 t1 a0 IHa0 a1 IHa1]; simpl in *; try reflexivity.
-        apply andb_true_iff in S; destruct S; rewrite IHa0, IHa1; try reflexivity; assumption.
-    Qed.
-  End Correctness.
-
-  Section FastCorrect.
     Context {n: nat}.
 
-    Record RangeWithValue := rwv {
-      low: N;
-      value: N;
-      high: N;
-    }.
+    Definition W := (word n).
+    Definition B := (@Bounded n).
+    Definition R := (option RangeWithValue).
 
-    Definition rwv_app {rangeF wordF}
-      (op: @validBinaryWordOp n rangeF wordF)
-      (X Y: RangeWithValue): option (RangeWithValue) :=
-      omap (rangeF (range N (low X) (high X)) (range N (low Y) (high Y))) (fun r' =>
-        match r' with
-        | range l h => Some (
-          rwv l (wordToN (wordF (NToWord n (value X)) (NToWord n (value Y)))) h)
-        end).
+    Instance RE : Evaluable R := @RWVEvaluable n.
+    Instance ZE : Evaluable Z := @ZEvaluable n.
+    Instance WE : Evaluable W := @WordEvaluable n.
+    Instance BE : Evaluable B := @BoundedEvaluable n.
 
-    Definition proj (x: RangeWithValue): Range N := range N (low x) (high x).
+    Transparent ZE RE WE BE W B R.
 
-    Definition from_range (x: Range N): RangeWithValue :=
-      match x with
-      | range l h => rwv l h h
-      end.
-
-    Instance RWVEval : Evaluable (option RangeWithValue) := {
-      ezero := None;
-
-      toT := fun x => 
-        if (Nge_dec (N.pred (Npow2 n)) (Z.to_N x))
-        then Some (rwv (Z.to_N x) (Z.to_N x) (Z.to_N x))
-        else None;
-
-      fromT := fun x => orElse 0%Z (option_map Z.of_N (option_map value x));
-
-      eadd := fun x y => omap x (fun X => omap y (fun Y =>
-        rwv_app range_add_valid X Y));
-
-      esub := fun x y => omap x (fun X => omap y (fun Y =>
-        rwv_app range_sub_valid X Y));
-
-      emul := fun x y => omap x (fun X => omap y (fun Y =>
-        rwv_app range_mul_valid X Y));
-
-      eshiftr := fun x y => omap x (fun X => omap y (fun Y =>
-        rwv_app range_shiftr_valid X Y));
-
-      eand := fun x y => omap x (fun X => omap y (fun Y =>
-        rwv_app range_and_valid X Y));
-
-      eltb := fun x y =>
-        match (x, y) with
-        | (Some (rwv xlow xv xhigh), Some (rwv ylow yv yhigh)) =>
-            N.ltb xv yv
-
-        | _ => false 
-        end;
-
-      eeqb := fun x y =>
-        match (x, y) with
-        | (Some (rwv xlow xv xhigh), Some (rwv ylow yv yhigh)) =>
-            andb (andb (N.eqb xlow ylow) (N.eqb xhigh yhigh)) (N.eqb xv yv)
-
-        | _ => false
-        end;
-    }.
-
-    Definition getRWV {t} T (E: Evaluable T) (e : @expr T T t): @interp_type (option RangeWithValue) t :=
-      interp (@convertExpr T (option RangeWithValue) E RWVEval t e).
-
-    Definition getRanges {t} T (E: Evaluable T) (e : @expr T T t): @interp_type (option (Range N)) t :=
-      typeMap (option_map proj) (getRWV T E e).
-
-    Fixpoint check' {t} (x: @interp_type (option RangeWithValue) t) :=
-      match t as t' return (interp_type t') -> bool with
-      | TT => fun x' =>
-        match x' with
-        | Some _ => true
-        | None => false
-        end
-      | Prod t0 t1 => fun x' =>
-        match x' with
-        | (x0, x1) => andb (check' x0) (check' x1)
-        end
-      end x.
-
-    Definition check {t} T (E: Evaluable T) (e : @expr T T t): bool :=
-      check' (getRWV T E e).
+    Existing Instance ZE.
+    Existing Instance RE.
+    Existing Instance WE.
+    Existing Instance BE.
 
     Ltac kill_dec :=
       repeat match goal with
@@ -414,68 +215,297 @@ Module LLConversions.
       | [H : context[Nge_dec ?a ?b] |- _ ] => destruct (Nge_dec a b)
       end.
 
-    Lemma check_spec: forall {t} (E: expr t),
-         check Z ZEvaluable E = true
-      -> bcheck (n := n) Z ZEvaluable E = true.
-    Proof.
-      intros t E H.
-      induction E as [tx ty tz op x y z eC IH| t a].
+    Section BoundsChecking.
+      Context {T: Type} {E: Evaluable T}.
 
-      - unfold bcheck, getBounds, check, getRWV in *.
-        apply IH; simpl in *; revert H; clear IH.
-        repeat rewrite convertArg_interp.
-        generalize (interp_arg x) as X; intro X; clear x.
-        generalize (interp_arg y) as Y; intro Y; clear y.
-        intro H; rewrite <- H; clear H; repeat f_equal.
+      Definition boundVarInterp := fun x => bwFromRWV (n := n) (rwv 0%N (Z.to_N x) (Z.to_N x)).
 
-        induction op; unfold ZEvaluable, BoundedEvaluable, RWVEval, just in *;
-          simpl in *; kill_dec; simpl in *; try reflexivity;
-          try rewrite (bapp_value_spec _ _ _ (fun x => Z.of_N (@wordToN n x)));
-          unfold vapp, rapp, rwv_app, overflows in *; kill_dec; simpl in *;
-          try reflexivity; try nomega.
+      Definition getBounds {t} (e : @expr T Z t): @interp_type B t :=
+        interp' boundVarInterp (@convertExpr T B _ _ t _ e).
 
-      - induction a as [c|v|t0 t1 a0 IHa0 a1 IHa1];
-          unfold bcheck, getBounds, check, getRWV in *; simpl in *; unfold just.
+      Fixpoint bcheck' {t} (x: @interp_type B t) :=
+        match t as t' return (interp_type t') -> bool with
+        | TT => fun x' =>
+          match x' with
+          | Some _ => true
+          | None => false
+          end
+        | Prod t0 t1 => fun x' =>
+          match x' with
+          | (x0, x1) => andb (bcheck' x0) (bcheck' x1)
+          end
+        end x.
 
-        + induction (Nge_dec (N.pred (Npow2 n)) (Z.to_N c));
-            simpl in *; [reflexivity|inversion H].
+      Definition bcheck {t} (e : expr t): bool := bcheck' (getBounds e).
+    End BoundsChecking.
 
-        + induction (Nge_dec (N.pred (Npow2 n)) (Z.to_N v));
-            simpl in *; [reflexivity|inversion H].
+    Section UtilityLemmas.
+      Context {A B} {EA: Evaluable A} {EB: Evaluable B}.
 
-        + apply andb_true_iff; apply andb_true_iff in H;
-            destruct H as [H0 H1]; split;
-            [apply IHa0|apply IHa1]; assumption.
-    Qed.
+      Lemma convertArg_interp' : forall {t V} f (x: @arg A V t),
+          (interp_arg' (fun z => toT (fromT (f z))) (@convertArg A B EA EB _ t x))
+            = @convertVar A B EA EB t (interp_arg' f x).
+      Proof.
+        intros.
+        induction x as [| |t0 t1 i0 i1]; simpl; [reflexivity|reflexivity|].
+        induction EA, EB; simpl; f_equal; assumption.
+      Qed.
 
-    Lemma RangeInterp_spec: forall {t} (E: expr t),
-        check Z ZEvaluable E = true
-      -> typeMap (fun x => NToWord n (Z.to_N x)) (zinterp E) = wordInterp (convertZToWord n E).
-    Proof.
-      intros.
-      apply RangeInterp_bounded_spec.
-      apply check_spec.
-      assumption.
-    Qed.
+      Lemma convertArg_var: forall {A B EA EB t} V (x: @interp_type A t),
+          @convertArg A B EA EB V t (uninterp_arg x) = uninterp_arg (var := V) (@convertVar A B EA EB t x).
+      Proof.
+        induction t as [|t0 IHt_0 t1 IHt_1]; simpl; intros; [reflexivity|].
+        induction x as [a b]; simpl; f_equal;
+            induction t0 as [|t0a IHt0_0 t0b IHt0_1],
+                    t1 as [|t1a IHt1_0]; simpl in *;
+            try rewrite IHt_0;
+            try rewrite IHt_1;
+            reflexivity.
+      Qed.
 
-    Lemma getRanges_spec: forall {t} T E (e: @expr T T t),
-      getRanges T E e = typeMap (t := t) (option_map (toRange (n := n))) (getBounds T E e).
-    Proof.
-      intros; induction e as [tx ty tz op x y z eC IH| t a];
-        unfold getRanges, getRWV, option_map, toRange, getBounds in *;
-        simpl in *.
+      Lemma ZToBounded_binop_correct : forall {tx ty tz} (op: binop tx ty tz) (x: @arg Z Z tx) (y: @arg Z Z ty) e,
+          bcheck (t := tz) (LetBinop op x y e) = true
+        -> opZ (n := n) op (interp_arg x) (interp_arg y) =
+          varBoundedToZ (n := n) (opBounded op
+             (interp_arg' boundVarInterp (convertArg _ x))
+             (interp_arg' boundVarInterp (convertArg _ y))).
+      Proof.
+      Admitted.
 
-      - rewrite <- IH; clear IH; simpl.
-        repeat f_equal.
-        repeat rewrite (convertArg_interp x); generalize (interp_arg x) as X; intro; clear x.
-        repeat rewrite (convertArg_interp y); generalize (interp_arg y) as Y; intro; clear y.
+      Lemma ZToWord_binop_correct : forall {tx ty tz} (op: binop tx ty tz) (x: arg tx) (y: arg ty) e,
+          bcheck (t := tz) (LetBinop op x y e) = true
+        -> opZ (n := n) op (interp_arg x) (interp_arg y) =
+            varWordToZ (opWord (n := n) op (varZToWord (interp_arg x)) (varZToWord (interp_arg y))).
+      Proof.
+      Admitted.
 
-        (* induction op;
-          unfold RWVEval, BoundedEvaluable, bapp, rwv_app,
-                 overflows, omap, option_map, just; simpl;
-          kill_dec; simpl in *. *)
-    Admitted.
-  End FastCorrect.
+      Lemma roundTrip_0 : @toT Correctness.B BE (@fromT Z ZE 0%Z) <> None.
+      Proof.
+        intros; unfold toT, fromT, BE, ZE, BoundedEvaluable, ZEvaluable, bwFromRWV;
+          kill_dec; simpl; kill_dec; simpl; try abstract (intro Z; inversion Z);
+          pose proof (Npow2_gt0 n); simpl in *; nomega.
+      Qed.
+
+      Lemma double_conv_var: forall t x,
+        @convertVar R Z _ _ t (@convertVar B R _ _ t x) =
+          @convertVar B Z _ _ t x.
+      Proof.
+        intros.
+      Admitted.
+
+      Lemma double_conv_arg: forall V t a,
+        @convertArg R B _ _ V t (@convertArg Z R _ _ V t a) =
+          @convertArg Z B _ _ V t a.
+      Proof.
+        intros.
+      Admitted.
+    End UtilityLemmas.
+
+
+    Section Spec.
+      Ltac kill_just n :=
+        match goal with
+        | [|- context[just ?x] ] =>
+            let Hvalue := fresh in let Hvalue' := fresh in
+            let Hlow := fresh in let Hlow' := fresh in
+            let Hhigh := fresh in let Hhigh' := fresh in
+            let Hnone := fresh in let Hnone' := fresh in
+
+            let B := fresh in
+
+            pose proof (just_value_spec (n := n) x) as Hvalue;
+            pose proof (just_low_spec (n := n) x) as Hlow;
+            pose proof (just_high_spec (n := n) x) as Hhigh;
+            pose proof (just_None_spec (n := n) x) as Hnone;
+
+            destruct (just x);
+
+            try pose proof (Hlow _ eq_refl) as Hlow';
+            try pose proof (Hvalue _ eq_refl) as Hvalue';
+            try pose proof (Hhigh _ eq_refl) as Hhigh';
+            try pose proof (Hnone eq_refl) as Hnone';
+
+            clear Hlow Hhigh Hvalue Hnone
+        end.
+
+      Lemma RangeInterp_bounded_spec: forall {t} (E: expr t),
+          bcheck (@convertExpr Z R _ _ _ _ E) = true
+        -> typeMap (fun x => NToWord n (Z.to_N x)) (zinterp (n := n) E) = wordInterp (ZToWord _ E).
+      Proof.
+        intros t E S.
+        unfold zinterp, ZToWord, wordInterp.
+
+        induction E as [tx ty tz op x y z|]; simpl; try reflexivity.
+
+        - repeat rewrite convertArg_var in *.
+          repeat rewrite convertArg_interp in *.
+
+          rewrite H; clear H; repeat f_equal.
+
+          + pose proof (ZToWord_binop_correct op x y) as C;
+              unfold opZ, opWord, varWordToZ, varZToWord in C;
+              simpl in C.
+
+            assert (N.pred (Npow2 n) >= 0)%N. {
+              apply N.le_ge.
+              rewrite <- (N.pred_succ 0).
+              apply N.le_pred_le_succ.
+              rewrite N.succ_pred; [| apply N.neq_0_lt_0; apply Npow2_gt0].
+              apply N.le_succ_l.
+              apply Npow2_gt0.
+            }
+
+            admit. (*
+            induction op; rewrite (C (fun _ => Return (Const 0%Z))); clear C;
+              unfold bcheck, getBounds, boundedInterp, bwFromRWV in *; simpl in *;
+              kill_dec; simpl in *; kill_dec; first [reflexivity|nomega]. *)
+
+          + unfold bcheck, getBounds in *.
+            replace (interp_binop op _ _)
+                with (varBoundedToZ (n := n) (opBounded op
+                        (interp_arg' boundVarInterp (convertArg _ x))
+                        (interp_arg' boundVarInterp (convertArg _ y)))).
+
+            * rewrite <- S; f_equal; clear S.
+              simpl; repeat f_equal.
+              unfold varBoundedToZ, opBounded.
+              repeat rewrite convertArg_var.
+              Arguments convertArg _ _ _ _ _ _ _ : clear implicits.
+              rewrite double_conv_var.
+              repeat rewrite double_conv_arg.
+              reflexivity.
+
+            * pose proof (ZToBounded_binop_correct op x y) as C;
+                unfold opZ, opWord, varZToBounded,
+                    varBoundedToZ in *;
+                simpl in C.
+
+              Local Opaque boundVarInterp toT fromT.
+
+              induction op; rewrite (C (fun _ => Return (Const 0%Z))); clear C; try reflexivity;
+                unfold bcheck, getBounds; simpl;
+                pose proof roundTrip_0 as H;
+                induction (toT (fromT _)); first [reflexivity|contradict H; reflexivity].
+
+              Local Transparent boundVarInterp toT fromT.
+
+        - simpl in S.
+          induction a as [| |t0 t1 a0 IHa0 a1 IHa1]; simpl in *; try reflexivity.
+          admit.
+
+          (*
+          + f_equal.
+            unfold bcheck, getBounds, boundedInterp in S; simpl in S.
+            kill_dec; simpl; [reflexivity|simpl in S; inversion S].
+
+          + f_equal.
+            unfold bcheck, getBounds, boundedInterp, boundVarInterp in S; simpl in S;
+              kill_dec; simpl; try reflexivity; try nomega.
+            inversion S.
+            admit.
+            admit.
+
+          + unfold bcheck in S; simpl in S;
+              apply andb_true_iff in S; destruct S as [S0 S1];
+              rewrite IHa0, IHa1; [reflexivity| |];
+              unfold bcheck, getBounds; simpl; assumption. *)
+      Admitted.
+    End Spec.
+
+    Section RWVSpec.
+      Definition rangeOf := fun x =>
+        Some (rwv 0%N (Z.to_N x) (Z.to_N x)).
+
+      Definition getRWV {t} (e : @expr R Z t): @interp_type R t :=
+        interp' rangeOf e.
+
+      Definition getRanges {t} (e : @expr R Z t): @interp_type (option (Range N)) t :=
+        typeMap (option_map rwvToRange) (getRWV e).
+
+      Fixpoint check' {t} (x: @interp_type (option RangeWithValue) t) :=
+        match t as t' return (interp_type t') -> bool with
+        | TT => fun x' =>
+            match omap x' (bwFromRWV (n := n)) with
+            | Some _ => true
+            | None => false
+            end
+        | Prod t0 t1 => fun x' =>
+            match x' with
+            | (x0, x1) => andb (check' x0) (check' x1)
+            end
+        end x.
+
+      Definition check {t} (e : @expr R Z t): bool := check' (getRWV e).
+
+      Ltac kill_dec :=
+        repeat match goal with
+        | [|- context[Nge_dec ?a ?b] ] => destruct (Nge_dec a b)
+        | [H : context[Nge_dec ?a ?b] |- _ ] => destruct (Nge_dec a b)
+        end.
+
+      Lemma check_spec' : forall {rangeF wordF} (op: @validBinaryWordOp n rangeF wordF) x y,
+        @convertVar B R _ _ TT (
+          omap (interp_arg' boundVarInterp (convertArg TT x)) (fun X =>
+            omap (interp_arg' boundVarInterp (convertArg TT y)) (fun Y =>
+              bapp op X Y))) =
+          omap (interp_arg' rangeOf x) (fun X =>
+            omap (interp_arg' rangeOf y) (fun Y =>
+              rwv_app (n := n) op X Y)).
+      Proof.
+      Admitted.
+
+      Lemma check_spec: forall {t} (E: @expr R Z t), check E = true -> bcheck E = true.
+      Proof.
+        intros t E H.
+        induction E as [tx ty tz op x y z eC IH| t a].
+
+        - unfold bcheck, getBounds, check, getRWV in *.
+
+          simpl; apply IH; clear IH; rewrite <- H; clear H.
+          simpl; rewrite convertArg_var; repeat f_equal.
+
+          unfold interp_binop, RE, WE, BE, ZE,
+              BoundedEvaluable, RWVEvaluable, ZEvaluable,
+              eadd, emul, esub, eshiftr, eand.
+
+          induction op; rewrite check_spec'; reflexivity.
+
+        - unfold bcheck, getBounds, check, getRWV in *.
+
+          induction a as [a|a|t0 t1 a0 IHa0 a1 IHa1].
+
+          + induction a as [a|]; [| inversion H]; simpl in *.
+
+            assert (Z : (exists a', bwFromRWV (n := n) a = Some a')
+                  \/ bwFromRWV (n := n) a = None) by (
+              destruct (bwFromRWV a);
+              [left; eexists; reflexivity | right; reflexivity]).
+
+            destruct Z as [aSome|aNone]; [destruct aSome as [a' aSome] |].
+
+            * rewrite aSome; simpl; rewrite aSome; reflexivity.
+            * rewrite aNone in H; inversion H.
+
+          + unfold boundVarInterp, rangeOf in *.
+            simpl in *; kill_dec; try reflexivity; try inversion H.
+
+          + simpl in *; rewrite IHa0, IHa1; simpl; [reflexivity | | ];
+              apply andb_true_iff in H; destruct H as [H1 H2];
+              assumption.
+      Qed.
+
+      Lemma RangeInterp_spec: forall {t} (E: expr t),
+          check (convertExpr E) = true
+        -> typeMap (fun x => NToWord n (Z.to_N x)) (zinterp (n := n) E)
+            = wordInterp (ZToWord _ E).
+      Proof.
+        intros.
+        apply RangeInterp_bounded_spec.
+        apply check_spec.
+        assumption.
+      Qed.
+    End RWVSpec.
+  End Correctness.
 End LLConversions.
 
 Section ConversionTest.
@@ -492,22 +522,22 @@ Section ConversionTest.
 
   Definition testCase := Eval vm_compute in KeepAddingOne 4000.
 
-  Eval vm_compute in (typeMap (option_map toRange) (BInterp (ZToRange 0 testCase))).
-  Eval vm_compute in (typeMap (option_map toRange) (BInterp (ZToRange 1 testCase))).
-  Eval vm_compute in (typeMap (option_map toRange) (BInterp (ZToRange 10 testCase))).
-  Eval vm_compute in (typeMap (option_map toRange) (BInterp (ZToRange 32 testCase))).
-  Eval vm_compute in (typeMap (option_map toRange) (BInterp (ZToRange 64 testCase))).
-  Eval vm_compute in (typeMap (option_map toRange) (BInterp (ZToRange 128 testCase))).
+  Eval vm_compute in (typeMap (option_map bwToRange) (BInterp (ZToRange 0 testCase))).
+  Eval vm_compute in (typeMap (option_map bwToRange) (BInterp (ZToRange 1 testCase))).
+  Eval vm_compute in (typeMap (option_map bwToRange) (BInterp (ZToRange 10 testCase))).
+  Eval vm_compute in (typeMap (option_map bwToRange) (BInterp (ZToRange 32 testCase))).
+  Eval vm_compute in (typeMap (option_map bwToRange) (BInterp (ZToRange 64 testCase))).
+  Eval vm_compute in (typeMap (option_map bwToRange) (BInterp (ZToRange 128 testCase))).
 
   Definition nefarious : Expr (T := Z) TT :=
     fun var => Let (Binop OPadd (Const 10%Z) (Const 20%Z))
                    (fun y => Binop OPmul (Var y) (Const 0%Z)).
 
-  Eval vm_compute in (typeMap (option_map toRange) (BInterp (ZToRange 0 nefarious))).
-  Eval vm_compute in (typeMap (option_map toRange) (BInterp (ZToRange 1 nefarious))).
-  Eval vm_compute in (typeMap (option_map toRange) (BInterp (ZToRange 4 nefarious))).
-  Eval vm_compute in (typeMap (option_map toRange) (BInterp (ZToRange 5 nefarious))).
-  Eval vm_compute in (typeMap (option_map toRange) (BInterp (ZToRange 32 nefarious))).
-  Eval vm_compute in (typeMap (option_map toRange) (BInterp (ZToRange 64 nefarious))).
-  Eval vm_compute in (typeMap (option_map toRange) (BInterp (ZToRange 128 nefarious))).
+  Eval vm_compute in (typeMap (option_map bwToRange) (BInterp (ZToRange 0 nefarious))).
+  Eval vm_compute in (typeMap (option_map bwToRange) (BInterp (ZToRange 1 nefarious))).
+  Eval vm_compute in (typeMap (option_map bwToRange) (BInterp (ZToRange 4 nefarious))).
+  Eval vm_compute in (typeMap (option_map bwToRange) (BInterp (ZToRange 5 nefarious))).
+  Eval vm_compute in (typeMap (option_map bwToRange) (BInterp (ZToRange 32 nefarious))).
+  Eval vm_compute in (typeMap (option_map bwToRange) (BInterp (ZToRange 64 nefarious))).
+  Eval vm_compute in (typeMap (option_map bwToRange) (BInterp (ZToRange 128 nefarious))).
 End ConversionTest.
