src/Assembly/GF25519.v
@@ -9,6 +9,9 @@ Module GF25519.
   Definition bits: nat := 64.
   Definition width: Width bits := W64.
 
+  Instance ZE : Evaluable Z := @ZEvaluable bits.
+  Existing Instance ZE.
+
   Fixpoint makeBoundList {n} k (b: @BoundedWord n) :=
     match k with
     | O => nil
@@ -17,9 +20,9 @@ Module GF25519.
 
   Section DefaultBounds.
     Import ListNotations.
-    Local Notation rr exp := (range N 0%N (2^exp + 2^exp/10)%N).
+    Local Notation rr exp := (2^exp + 2^exp/10)%Z.
 
-    Definition feBound: list (Range N) :=
+    Definition feBound: list Z :=
       [rr 26; rr 27; rr 26; rr 27; rr 26;
        rr 27; rr 26; rr 27; rr 26; rr 27].
   End DefaultBounds.
@@ -45,8 +48,7 @@ Module GF25519.
         Eval cbv beta delta [fe25519 add mul sub Let_In] in add.
 
     Definition ge25519_add' (P Q: @interp_type Z FE) :
-        { r: @HL.expr Z (@interp_type Z) FE
-        | HL.interp (E := ZEvaluable) (t := FE) r = ge25519_add_expr P Q }.
+        { r: @HL.expr Z (@interp_type Z) FE | HL.interp (t := FE) r = ge25519_add_expr P Q }.
     Proof.
       vm_compute in P, Q; repeat
         match goal with
@@ -63,8 +65,7 @@ Module GF25519.
 
       let R := HL.rhs_of_goal in
       let X := HL.reify (@interp_type Z) R in
-      transitivity (HL.interp (E := ZEvaluable) (t := ResultType) X);
-        [reflexivity|].
+      transitivity (HL.interp (t := ResultType) X); [reflexivity|].
 
       cbv iota beta delta [
             interp_type interp_binop HL.interp
@@ -75,123 +76,9 @@ Module GF25519.
     Definition ge25519_add (P Q: @interp_type Z ResultType) :=
         proj1_sig (ge25519_add' P Q).
 
-    Definition hlProg'': NAry 20 Z (@HL.expr Z (@interp_type Z) ResultType) :=
+    Definition hlProg: NAry 20 Z (@HL.expr Z (@interp_type Z) ResultType) :=
         liftFE (fun p => (liftFE (fun q => ge25519_add p q))).
-
-    Definition hlProg': NAry 20 Z (@HL.expr Z (@LL.arg Z Z) ResultType).
-        refine (liftN (HLConversions.mapVar _ _) hlProg''); intro t;
-        [ refine LL.uninterp_arg | refine LL.interp_arg ].
-    Defined.
-
-    Definition hlProg: NAry 20 Z (@HL.expr Z (@LL.arg Z Z) ResultType) :=
-      Eval vm_compute in hlProg'.
   End AddExpr.
-
-  Module SubExpr <: Expression.
-    Definition bits: nat := bits.
-    Definition inputs: nat := 20.
-    Definition width: Width bits := width.
-    Definition ResultType := FE.
-    Definition inputBounds := feBound ++ feBound.
-
-    Definition ge25519_sub_expr :=
-        Eval cbv beta delta [fe25519 add mul sub Let_In] in sub.
-
-    Definition ge25519_sub' (P Q: @interp_type Z FE) :
-        { r: @HL.expr Z (@interp_type Z) FE
-        | HL.interp (E := ZEvaluable) (t := FE) r = ge25519_sub_expr P Q }.
-    Proof.
-      vm_compute in P, Q; repeat
-        match goal with
-        | [x:?T |- _] =>
-          lazymatch T with
-          | Z => fail
-          | prod _ _ => destruct x
-          | _ => clear x
-          end
-        end.
-
-      eexists.
-      cbv beta delta [ge25519_sub_expr].
-
-      let R := HL.rhs_of_goal in
-      let X := HL.reify (@interp_type Z) R in
-      transitivity (HL.interp (E := ZEvaluable) (t := ResultType) X);
-        [reflexivity|].
-
-      cbv iota beta delta [
-        interp_type interp_binop HL.interp
-        Z.land ZEvaluable eadd esub emul eshiftr eand].
-      reflexivity.
-    Defined.
-
-    Definition ge25519_sub (P Q: @interp_type Z ResultType) :=
-        proj1_sig (ge25519_sub' P Q).
-
-    Definition hlProg'': NAry 20 Z (@HL.expr Z (@interp_type Z) ResultType) :=
-        liftFE (fun p => (liftFE (fun q => ge25519_sub p q))).
-
-    Definition hlProg': NAry 20 Z (@HL.expr Z (@LL.arg Z Z) ResultType).
-        refine (liftN (HLConversions.mapVar _ _) hlProg''); intro t;
-        [ refine LL.uninterp_arg | refine LL.interp_arg ].
-    Defined.
-
-    Definition hlProg: NAry 20 Z (@HL.expr Z (@LL.arg Z Z) ResultType) :=
-      Eval vm_compute in hlProg'.
-  End SubExpr.
-
-  Module MulExpr <: Expression.
-    Definition bits: nat := bits.
-    Definition inputs: nat := 20.
-    Definition width: Width bits := width.
-    Definition ResultType := FE.
-    Definition inputBounds := feBound ++ feBound.
-
-    Definition ge25519_mul_expr :=
-        Eval cbv beta delta [fe25519 add mul sub Let_In] in mul.
-
-    Definition ge25519_mul' (P Q: @interp_type Z FE) :
-        { r: @HL.expr Z (@interp_type Z) FE
-        | HL.interp (E := ZEvaluable) (t := FE) r = ge25519_mul_expr P Q }.
-    Proof.
-      vm_compute in P, Q; repeat
-        match goal with
-        | [x:?T |- _] =>
-          lazymatch T with
-          | Z => fail
-          | prod _ _ => destruct x
-          | _ => clear x
-          end
-      end.
-
-      eexists.
-      cbv beta delta [ge25519_mul_expr].
-
-      let R := HL.rhs_of_goal in
-      let X := HL.reify (@interp_type Z) R in
-      transitivity (HL.interp (E := ZEvaluable) (t := ResultType) X);
-        [reflexivity|].
-
-      cbv iota beta delta [
-        interp_type interp_binop HL.interp
-        Z.land ZEvaluable eadd esub emul eshiftr eand].
-      reflexivity.
-    Defined.
-
-    Definition ge25519_mul (P Q: @interp_type Z ResultType) :=
-        proj1_sig (ge25519_mul' P Q).
-
-    Definition hlProg'': NAry 20 Z (@HL.expr Z (@interp_type Z) ResultType) :=
-        liftFE (fun p => (liftFE (fun q => ge25519_mul p q))).
-
-    Definition hlProg': NAry 20 Z (@HL.expr Z (@LL.arg Z Z) ResultType).
-        refine (liftN (HLConversions.mapVar _ _) hlProg''); intro t;
-        [ refine LL.uninterp_arg | refine LL.interp_arg ].
-    Defined.
-
-    Definition hlProg: NAry 20 Z (@HL.expr Z (@LL.arg Z Z) ResultType) :=
-      Eval vm_compute in hlProg'.
-  End MulExpr.
 
   Module OppExpr <: Expression.
     Definition bits: nat := bits.
@@ -205,7 +92,7 @@ Module GF25519.
 
     Definition ge25519_opp' (P: @interp_type Z FE) :
         { r: @HL.expr Z (@interp_type Z) FE
-        | HL.interp (E := ZEvaluable) (t := FE) r = ge25519_opp_expr P }.
+        | HL.interp (E := @ZEvaluable bits) (t := FE) r = ge25519_opp_expr P }.
     Proof.
       vm_compute in P; repeat
         match goal with
@@ -222,7 +109,7 @@ Module GF25519.
 
       let R := HL.rhs_of_goal in
       let X := HL.reify (@interp_type Z) R in
-      transitivity (HL.interp (E := ZEvaluable) (t := ResultType) X);
+      transitivity (HL.interp (E := @ZEvaluable bits) (t := ResultType) X);
         [reflexivity|].
 
       cbv iota beta delta [
@@ -234,25 +121,41 @@ Module GF25519.
     Definition ge25519_opp (P: @interp_type Z ResultType) :=
         proj1_sig (ge25519_opp' P).
 
-    Definition hlProg'': NAry 10 Z (@HL.expr Z (@interp_type Z) ResultType) :=
+    Definition hlProg: NAry 10 Z (@HL.expr Z (@interp_type Z) ResultType) :=
         liftFE (fun p => ge25519_opp p).
-
-    Definition hlProg': NAry 10 Z (@HL.expr Z (@LL.arg Z Z) ResultType).
-        refine (liftN (HLConversions.mapVar _ _) hlProg''); intro t;
-        [ refine LL.uninterp_arg | refine LL.interp_arg ].
-    Defined.
-
-    Definition hlProg: NAry 10 Z (@HL.expr Z (@LL.arg Z Z) ResultType) :=
-      Eval vm_compute in hlProg'.
   End OppExpr.
 
   Module Add := Pipeline AddExpr.
-  Module Sub := Pipeline SubExpr.
-  Module Mul := Pipeline MulExpr.
   Module Opp := Pipeline OppExpr.
+
+  Section Operations.
+    Definition wfe: Type := @interp_type (word bits) FE.
+
+    Definition ExprBinOp : Type := NAry 20 Z (@CompileLL.WExpr bits FE).
+    Definition ExprUnOp : Type := NAry 10 Z (@CompileLL.WExpr bits FE).
+
+    Existing Instance WordEvaluable.
+
+    Definition interp_bexpr (op: ExprBinOp) (x y: tuple (word bits) 10): tuple (word bits) 10 :=
+      let '(x0, x1, x2, x3, x4, x5, x6, x7, x8, x9) := x in 
+      let '(y0, y1, y2, y3, y4, y5, y6, y7, y8, y9) := y in
+      let op' := NArgMap (fun v => Z.of_N (@wordToN bits v)) op in
+      let z := LL.interp (op' x0 x1 x2 x3 x4 x5 x6 x7 x8 x9 y0 y1 y2 y3 y4 y5 y6 y7 y8 y9) in
+        z.
+
+    Definition interp_uexpr (op: ExprUnOp) (x: tuple (word bits) 10): tuple (word bits) 10 :=
+      let '(x0, x1, x2, x3, x4, x5, x6, x7, x8, x9) := x in 
+      let op' := NArgMap (fun v => Z.of_N (@wordToN bits v)) op in
+      let z := LL.interp (op' x0 x1 x2 x3 x4 x5 x6 x7 x8 x9) in
+        z.
+ 
+    Definition radd : ExprBinOp := Add.wordProg.
+    Definition ropp : ExprUnOp := Opp.wordProg.
+  End Operations.
 End GF25519.
 
 Extraction "GF25519Add" GF25519.Add.
 Extraction "GF25519Sub" GF25519.Sub.
 Extraction "GF25519Mul" GF25519.Mul.
 Extraction "GF25519Opp" GF25519.Opp.
+
